src/Narcissus/Examples/Guard/PacketFiltersLemmas.v
@@ -1,5 +1,6 @@
 Require Import
         Coq.Lists.List
+        Coq.Sorting.Permutation
         Fiat.Computation
         Fiat.ADT
         Fiat.ADTRefinement
@@ -23,7 +24,8 @@ Require Import
         Fiat.QueryStructure.Automation.Common
         Fiat.QueryStructure.Automation.General.QueryAutomation
         Fiat.QueryStructure.Automation.General.InsertAutomation
-        Fiat.QueryStructure.Automation.General.DeleteAutomation.
+        Fiat.QueryStructure.Automation.General.DeleteAutomation
+        Fiat.Narcissus.Examples.Guard.DropFields.
 Import ListNotations.
 
         
@@ -55,14 +57,38 @@ Definition UnIndexedEnsembleListEquivalence'
             In IndexedElement ensemble x <-> List.In x l') /\
          NoDup (map elementIndex l')).
 
+
 Definition AllFinite {qs_schema} (r: UnConstrQueryStructure qs_schema) :=
-  forall idx, {l: list RawTuple & UnIndexedEnsembleListEquivalence' (GetUnConstrRelation r idx) l}.
+  forall idx, {l: list RawTuple & UnIndexedEnsembleListEquivalence' _ (GetUnConstrRelation r idx) l}.
 
 Definition FiniteTables_AbsR'
     {qs_schema}
     (r_o : UnConstrQueryStructure qs_schema)
     (r_n : { r_n: UnConstrQueryStructure qs_schema & AllFinite r_n }) :=
   r_o = projT1 r_n.
+
+Open Scope list.
+Lemma QSEmptyFinite {qs_schema}:
+  forall idx, FiniteEnsemble (GetUnConstrRelation (DropQSConstraints (QSEmptySpec qs_schema)) idx).
+Proof.
+  intros. red. exists []. red. exists [].
+  split.
+  - reflexivity.
+  - split.
+    * split; intros.
+      + cbn in H. red in H. red in H.
+        change (Vector.map schemaRaw (QSschemaSchemas qs_schema))
+          with (qschemaSchemas qs_schema) in H. rewrite <- ith_imap2 in H.
+        remember (ith2 _ _) in *.
+        change (numQSschemaSchemas qs_schema)
+          with (numRawQSschemaSchemas (QueryStructureSchemaRaw qs_schema)) in Heqy.
+        change (fun x => ?f x) with f in Heqy.
+
+        rewrite (Build_EmptyRelation_IsEmpty qs_schema idx) in Heqy.
+        subst y. cbn in H. inversion H.
+      + inversion H.
+    * constructor.
+Qed.
 
 Lemma QSEmptyIsFinite {qs_schema}: AllFinite (DropQSConstraints (QSEmptySpec qs_schema)).
 Proof.
@@ -84,6 +110,7 @@ Proof.
       + inversion H.
     * constructor.
 Qed.
+Close Scope list.
 
 Lemma FiniteTables_AbsR'_QSEmptySpec
       {qs_schema}
@@ -116,6 +143,7 @@ Proof.
   apply Return_inv in H. subst. apply IncrMaxFreshIdx_Prop.
 Qed.
 
+Open Scope list.
 Lemma insert_finite_helper:
   forall (qs_schema : RawQueryStructureSchema)
          (r_n: { r_n: UnConstrQueryStructure qs_schema & AllFinite r_n })
@@ -169,7 +197,7 @@ Lemma FiniteTables_AbsR'_Insert :
       (ret (existT AllFinite
               (UpdateUnConstrRelation (projT1 r_n) idx
                  (EnsembleInsert tup (GetUnConstrRelation (projT1 r_n) idx)))
-              (insert_finite_helper r_n idx tup H))).
+              (insert_finite_helper _ r_n idx tup H))).
 Proof.
   intros qsc r_n idx tup Hfreshn.
   unfold refine; intros r_n' Hr_n'. apply Return_inv in Hr_n'. subst r_n'.
@@ -177,7 +205,199 @@ Proof.
 Qed.
 
 
-Transparent QSInsert.
+Lemma simpl_in_bind:
+  forall (T U: Type) (x v : T) (y: U),
+    In T (`(r', _) <- ret (x, y); ret r') v -> x = v.
+Proof.
+  intros. apply Bind_inv in H. destruct H. destruct H. apply Return_inv in H. rewrite <- H in H0. simpl in H0. apply Return_inv in H0. assumption. Qed.
+
+Definition UnConstrQuery_In {ResultT}
+           {qsSchema}
+           (qs : UnConstrQueryStructure qsSchema)
+           (R : Fin.t _)
+           (bod : RawTuple -> Comp (list ResultT))
+  := QueryResultComp (GetUnConstrRelation qs R) bod.
+
+Notation "( x 'in' r '%' Ridx ) bod" :=
+  (let qs_schema : QueryStructureSchema := _ in
+   let r' : UnConstrQueryStructure qs_schema := r in
+   let Ridx' := ibound (indexb (@Build_BoundedIndex _ _ (QSschemaNames qs_schema) Ridx%string _)) in
+   @UnConstrQuery_In _ qs_schema r' Ridx'
+            (fun x : @RawTuple (GetNRelSchemaHeading (qschemaSchemas qs_schema) Ridx') => bod)) (at level 0, x at level 200, r at level 0, bod at level 0).
+
+Lemma permutation_length {A: Type}:
+  forall (l1 l2 : list A),
+    Permutation l1 l2 -> Datatypes.length l1 = Datatypes.length l2.
+Proof.
+  intros. induction H; simpl; congruence.
+Qed.
+
+Lemma fold_comp_list_in:
+  forall (T: Type) (P: T -> bool) (ltup: list T) l inp,
+    fold_right
+      (fun b a : Comp (list ()) =>
+         l <- b;
+         l' <- a;
+         ret (l ++ l')%list) (ret [])
+      (map
+         (fun t : T =>
+            {l : list () |
+             (P t -> ret [()] ↝ l) /\ (~ P t -> l = [])}) ltup) l ->
+    List.In inp ltup ->
+    P inp ->
+    0 <? Datatypes.length l.
+Proof.
+  intros T P. induction ltup.
+  - intros; auto.
+  - intros l inp Hf Hin Hp. cbn in Hf.  destruct Hf as [x [Hx [y [Hy Happ]]]].
+    unfold In in *. inversion Happ. destruct Hin as [Hin | Hin].
+    * subst inp. inversion Hx. apply H0 in Hp. inversion Hp. auto.
+    * pose proof (IHltup y inp Hy Hin Hp) as Hind. rewrite app_length.
+      apply Nat.ltb_lt; apply Nat.lt_lt_add_l; apply Nat.ltb_lt; assumption.
+Qed.
+
+Lemma fold_comp_list_length:
+  forall l l',
+    fold_right
+      (fun b a : Comp (list ()) =>
+         l <- b;
+         l' <- a;
+         ret (l ++ l')%list) (ret [])
+      l' l ->
+    0 <? Datatypes.length l ->
+    exists lin, List.In lin l' /\
+                (exists lin', lin lin' /\ 0 <? Datatypes.length lin').
+Proof.
+  intros l l'. generalize dependent l. induction l'.
+  - simpl. intros. inversion H. subst l. inversion H0.
+  - simpl. intros. destruct H as [l1 [Hl1 Hl]]. red in Hl1. red in Hl.
+    destruct Hl as [l2 [Hl2 Hl]]. red in Hl2. red in Hl. inversion Hl.
+    destruct (0 <? Datatypes.length l2) eqn:Hlen2.
+    * pose proof (IHl' l2 Hl2 Hlen2) as IH.
+      destruct IH as [lin [Hlin1 Hlin2]]. exists lin. split.
+      right; assumption. assumption.
+    * apply Nat.ltb_ge in Hlen2. inversion Hlen2. rewrite <- H in H0.
+      rewrite app_length in H0. rewrite H2 in H0. rewrite Nat.add_0_r in H0.
+      exists a. split.
+      left; reflexivity. exists l1. split. assumption. rewrite H2. apply H0.
+Qed.
+Close Scope list.
+
+Lemma count_zero_iff:
+  forall h (topkt: @Tuple h -> input) totup
+    (r: UnConstrQueryStructure (PacketHistorySchema h))
+    (P: input -> bool) count,
+    (forall t, totup (topkt t) = t) ->
+    (forall inp, P inp = P (topkt (totup inp))) ->
+    computes_to (Count (For (UnConstrQuery_In r Fin.F1
+                        (fun t =>
+                          Where (P (topkt t))
+                          Return ())))) count ->
+    ((0 <? count) <-> (exists inp, In_History totup r inp /\ P inp)).
+Proof.
+  Transparent Query_For. Transparent Count. Transparent QueryResultComp.
+  unfold Count, Query_For, Query_Where, Query_Return, UnConstrQuery_In.
+  unfold QueryResultComp, FlattenCompList.flatten_CompList.
+  intros h topkt totup r P count toinv Ptoinv Hcount.
+  destruct Hcount as [l [Hcount Htmp]].
+  unfold In in *. inversion Htmp. rename H into Hlen. clear Htmp.
+  destruct Hcount as [l' [Htmp Hperm]]. apply Pick_inv in Hperm.
+  unfold In in *. destruct Htmp as [ltup [Hrel Hfold]].
+  apply Pick_inv in Hrel. unfold In in *.
+  pose proof (permutation_length l' l Hperm) as Hpermlen.
+  rewrite <- Hpermlen in *. clear Hperm. clear Hpermlen. clear l.
+  split; intros H.
+  - pose proof (fold_comp_list_length l' _ Hfold H) as Hlin0.
+    destruct Hlin0 as [lin [Hlinm [lin' [Hll Hlinc]]]].
+    apply in_map_iff in Hlinm. destruct Hlinm as [x [Hpx Hlx]].
+    exists (topkt x). split.
+    * red in Hrel. destruct Hrel as [l [Hmap [Heql Hdup]]].
+      red. rewrite <- Hmap in Hlx.
+      apply in_map_iff in Hlx.
+      destruct Hlx as [y [Hy1 Hy2]]. destruct y as [yidx yelem].
+      exists yidx. simpl in Hy1. subst x. apply Heql. rewrite toinv. apply Hy2.
+    * subst lin. inversion Hll.
+      destruct (P (topkt x)) eqn:Hpx. reflexivity.
+      assert (Hle: lin' = []%list) by (apply H1; congruence). subst lin'.
+      inversion Hlinc.
+
+  - red in Hrel. destruct Hrel as [l [Hmap [Heql Hdup]]].
+    destruct H as [inp [Hinp Hpinp]]. red in Hinp. destruct Hinp as [idx Hinp].
+    apply Heql in Hinp.
+    assert (Hinp': List.In (totup inp) ltup).
+    { rewrite <- Hmap. apply in_map_iff.
+      exists {| elementIndex := idx; indexedElement := (totup inp) |}.
+      split. reflexivity. assumption. }
+    pose (fun t => P (topkt t)) as P'. rewrite Ptoinv in Hpinp.
+    apply (fold_comp_list_in _ P' ltup l' _ Hfold Hinp' Hpinp).
+Qed.
+
+Lemma list_helper:
+  forall {T: Type} (l: list T) (f: T -> nat) (big: nat),
+    lt (fold_right (fun e acc => max (f e) acc) 0 l) big ->
+    ~ List.In big (map f l).
+Proof.
+  induction l.
+  - auto.
+  - unfold not; intros f big Hbig H. cbn in Hbig. cbn in H.
+    pose proof
+         (Nat.max_spec (f a)
+                       (fold_right (fun (e : T) (acc : nat) =>
+                                      Init.Nat.max (f e) acc) 0 l)) as Hmax.
+    destruct Hmax as [[Hlt Hmax] | [Hlt Hmax]]; rewrite Hmax in Hbig;
+      destruct H as [H | H].
+    + subst big. pose proof (lt_trans _ _ _ Hlt Hbig).
+      apply lt_irrefl in H. auto.
+    + apply (IHl f big Hbig H).
+    + subst big. apply lt_irrefl in Hbig. auto.
+    + pose proof (le_lt_trans _ _ _ Hlt Hbig). apply (IHl f big H0 H).
+Qed.
+
+Lemma refine_pair: forall (T U: Type) (x: T) (y: U) (c: Comp T),
+    refine c (ret x) ->
+    refine
+      (x' <- c;
+         ret (x', y))
+      (ret (x, y)).
+Proof.
+  intros. intro; intros. comp_inv. computes_to_econstructor.
+  red in H. apply H. auto. auto. Qed.
+
+
+Definition StatefulFilterSig : ADTSig :=
+  ADTsignature {
+      Constructor "Init" : rep,
+      Method "Filter" : rep * input -> rep * (option result)
+    }.
+
+
+Ltac prove_count_refine :=
+  intros r inp;
+  match goal with
+  | [|- refine (?f1 _ _ _ _ _) (?f2 _ _ _ _ _)] => unfold f1, f2
+  end;
+  red; intros v H;
+  repeat match goal with
+  | [|- (If ?cond Then (ret _) Else _) ↝ _] =>
+    destruct cond; [ assumption | ]; simpl
+  | [H: (_ ↝ _) |- (with _ _, if historically _ then _ else _) ↝ _] =>
+    inversion H as [c Hc]; destruct Hc as [Hcount Hres]; unfold In in *;
+    pose 1 as Hcziff; clear Hcziff;
+    unshelve epose proof (count_zero_iff _ _ _ _ _ c _ _ Hcount) as Hcziff;
+    shelve_unifiable; cycle -1;
+    [ computes_to_econstructor; computes_to_econstructor;
+      [ instantiate (1:=(0 <? c)); red; destruct (0 <? c) eqn:Hzero; simpl;
+        [ rewrite <- Hzero in Hcziff; apply Hcziff in Hzero;
+          destruct Hzero as [pre [Hin Hcond]]; exists pre; split;
+          [ apply Hin | apply Hcond ]
+        | let H := fresh in
+          intro H; rewrite <- Hzero in Hcziff; apply Hcziff in H; congruence ]
+      | apply Hres ]
+    | intros t; repeat (let i := fresh in destruct t as [i t]); reflexivity
+    | reflexivity ]
+  end.
+
+
 Ltac drop_constraints_under_bind_insert :=
   unfold QSInsert;
   rewrite QSInsertSpec_UnConstr_refine; eauto; cycle 1;
@@ -216,8 +436,6 @@ Ltac drop_constraints_under_bind qs_schema bound_meth_tac :=
          ]
        ]
      end).
-
-
 
 Ltac hone_finite_under_bind_constructor :=
   match goal with
@@ -259,4 +477,26 @@ Ltac hone_finite_under_bind qs_schema idx :=
           | [|- pointwise_relation _ refine _ _] =>
             hone_finite_under_bind_insert qs_schema idx
           end)
-  end).
+   end).
+
+
+(** Tactics for generating variants of filters **)
+
+Ltac filter_gen gen :=
+  red; intros h topkt totup r inp;
+  let f := (eval unfold gen in @gen) in
+  let f' := (eval cbv beta in (@f h _ In_History topkt totup r inp)) in
+  apply f'.
+
+Ltac filter_count filter :=
+  red; intros h topkt totup r inp;
+  pose (filter h topkt totup r inp) as f; unfold filter in f;
+  repeat let f' := (eval unfold f in f) in
+  match f' with
+  | If ?cond Then (ret _) Else _ => destruct cond; [ apply f | ]; cbn in f
+  | with ?r ?cont, if historically ?cond then ?iftru else ?iffal =>
+    pose (c <- Count (For (t in r%"History")
+                       Where (cond (topkt t))
+                       Return ());
+           If 0 <? c Then iftru Else iffal) as hist_count; apply hist_count
+  end.
