src/Narcissus/Examples/Guard/BasicConnectionsFilter.v
@@ -1,0 +1,136 @@
+Require Import
+    Fiat.Narcissus.Examples.NetworkStack.IPv4Header
+    Fiat.Narcissus.Examples.NetworkStack.TCP_Packet
+    Bedrock.Word
+    Coq.Arith.Arith
+    Coq.Lists.List
+    Fiat.QueryStructure.Automation.MasterPlan
+    IndexedEnsembles
+    Fiat.Narcissus.Examples.Guard.IPTables
+    Fiat.Narcissus.Examples.Guard.PacketFiltersLemmas
+    Fiat.Narcissus.Examples.Guard.DropFields.
+Import ListNotations.
+
+(* TODO: Add a proper makefile target *)
+
+(**
+we are 18.X.X.X
+outside world is all other IP addresses
+filter allows outside address to talk to us only if we have talked to it first
+**)
+
+Definition OutgoingRule :=
+  iptables -A FORWARD --source 18'0'0'0/24.
+
+Definition IncomingRule :=
+  iptables -A FORWARD --destination 18'0'0'0/24.
+
+Definition OutgoingToRule (dst: address) :=
+  iptables -A FORWARD --source 18'0'0'0/24
+           --destination (Build_address_spec dst (mask_of_nat 32)).
+
+Definition OutgoingToRule' (cur pre : input) : Prop :=
+  (OutgoingToRule cur.(in_ip4).(SourceAddress)).(cf_cond) pre = true.
+
+Opaque OutgoingRule IncomingRule OutgoingToRule OutgoingToRule'.
+
+
+Definition FilterMethodGen {h T} cont
+           (topkt: @Tuple h -> input)
+           (totup: input -> @Tuple h)
+           (r: T) (inp: input) :=
+  If OutgoingRule.(cf_cond) inp
+  Then <ACCEPT>
+  Else (
+      If negb (IncomingRule.(cf_cond) inp)
+      Then ret None
+      Else with r (cont totup),
+                if historically (OutgoingToRule' inp) then <ACCEPT> else <DROP>).
+Definition FilterMethod: FilterType. filter_gen @FilterMethodGen. Defined.
+Definition FilterMethod_Count: FilterType. filter_count FilterMethod. Defined.
+
+Transparent computes_to.
+Theorem DroppedFilterMethod : FilterAdapter (@FilterMethod).
+Proof. solve_drop_fields @FilterMethod. Defined.
+Definition myh := (h _ DroppedFilterMethod).
+Definition mytopkt := (topkt _ DroppedFilterMethod).
+Definition mytotup := (totup _ DroppedFilterMethod).
+Definition mythm := (thm _ DroppedFilterMethod).
+
+Lemma CompPreservesFilterMethod:
+  forall r inp,
+    refine (FilterMethod myh mytopkt mytotup r inp)
+           (FilterMethod_Count myh mytopkt mytotup r inp).
+Proof. prove_count_refine. Qed.
+
+
+Definition NoIncomingConnectionsFilter : ADT StatefulFilterSig :=
+  Eval simpl in Def ADT {
+    rep := QueryStructure Complete_PacketHistorySchema,
+    Def Constructor0 "Init" : rep := empty,,
+
+    Def Method1 "Filter" (r: rep) (inp: input) : rep * option result :=
+      res <- FilterMethodGen In_History_Constr Complete_topkt Complete_totup r inp;
+      `(r, _) <- Insert (Complete_totup inp) into r!"History";
+      ret (r, res)
+  }%methDefParsing.
+
+Theorem SharpenNoIncomingFilter:
+  FullySharpened NoIncomingConnectionsFilter.
+Proof.
+  start sharpening ADT.
+
+  Transparent QSInsert.
+  drop_constraints_under_bind Complete_PacketHistorySchema ltac:(
+    instantiate (1:=(FilterMethodGen In_History Complete_topkt Complete_totup r_n d));
+    unfold FilterMethodGen; red; intros v Hv; red in Hv; red;
+
+    repeat match goal with
+    | [H: (If _ Then _ Else _) v |- (If ?cond Then _ Else _) v] =>
+      destruct cond; [ apply H | cbn; cbn in H ]
+    | [Hv: _ v |- _ v] => repeat comp_inv; apply Pick_inv in H1;
+                          repeat computes_to_econstructor; [ | eassumption ]
+    | [H: decides ?b _ |- _] => destruct b; cbn in *
+    | [H: exists pre, ?A /\ ?B |- exists _, _ /\ _] =>
+      destruct H as [pre [Ha Hb]]; exists pre; split; [ | assumption ]
+    | [Hrel: DropQSConstraints_AbsR ?r_o ?r_n, Hhist: In_History _ _ _ |- _] =>
+      unfold In_History, In_History_Constr, GetRelationBnd, GetUnConstrRelationBnd in *;
+      rewrite <- (GetRelDropConstraints r_o); rewrite <- Hrel in Hhist; apply Hhist
+    | [H: ~ _ |- ~ _] => intro; apply H
+    | [Hrel: DropQSConstraints_AbsR ?r_o ?r_n, Hhist: In_History_Constr _ _ _ |- _] =>
+      unfold In_History; rewrite <- Hrel; red in Hhist; unfold GetRelationBnd in Hhist;
+      rewrite <- (GetRelDropConstraints r_o) in Hhist; apply Hhist
+    end).
+
+  hone representation using (Complete_Dropped_qs_equiv mytotup);
+    try simplify with monad laws;
+  [ refine pick val (DropQSConstraints (QSEmptySpec _));
+    [ subst H; reflexivity
+    | red; intros; split; intros Htmp; cbv in Htmp; inversion Htmp]
+  | eapply refine_bind; [ apply mythm; apply H0 | intro res; cbn ];
+    eapply refine_bind; [ apply (DropPreservesFreshIdx _ _ _ mytotup H0)
+                        | intro idx; cbn ];
+    apply refine_pair; apply refine_pick; intros qs Hins; comp_inv; subst qs;
+    instantiate (1 := (UpdateUnConstrRelation r_n Fin.F1
+                         (BuildADT.EnsembleInsert
+                            {| elementIndex := idx;
+                               indexedElement := mytotup d |}
+                            (GetUnConstrRelation r_n Fin.F1))));
+
+    red; intros oinp oidx; split; intros Hoinp; destruct Hoinp as [Hoinp | Hoinp];
+    [ apply in_ensemble_insert_iff; left; inversion Hoinp; reflexivity
+    | right; apply H0 in Hoinp; apply Hoinp
+    | exists d; split; [ apply in_ensemble_insert_iff; left | ];
+      inversion Hoinp; reflexivity
+    | pose proof (H0 oinp oidx) as H0spec;
+      destruct H0spec as [_ Hspec]; specialize (Hspec Hoinp);
+      destruct Hspec as [inp' [H1 H2]]; exists inp'; split;
+      [ apply in_ensemble_insert_iff; right; apply H1 | apply H2 ]
+    ]
+  | ].
+
+
+ - hone method "Filter".
+   subst r_o; refine pick eq; simplify with monad laws;
+   apply refine_bind; [ apply CompPreservesFilterMethod; reflexivity | intro ];
+   apply refine_bind; [ reflexivity | intro; simpl; higher_order_reflexivity ].
